Define prefix for tock and prove healthiness

CTockTick_Prefix.thy
@@ -3,13 +3,11 @@ theory CTockTick_Prefix
 begin
 
 subsection {* Prefix *}
-  
 
 definition PrefixCTT :: "'e \<Rightarrow> 'e cttobs list set \<Rightarrow> 'e cttobs list set" (infixr "\<rightarrow>\<^sub>C" 61) where
   "PrefixCTT e P = 
     {t. \<exists> s\<in>tocks({x. x \<noteq> Tock \<and> x \<noteq> Event e}). t = s \<or> (\<exists> X. Tock \<notin> X \<and> Event e \<notin> X \<and> t = s @ [[X]\<^sub>R])}
      \<union> {t. \<exists> s\<in>tocks({x. x \<noteq> Tock \<and> x \<noteq> Event e}). t = s \<or> (\<exists> \<sigma>\<in>P. t = s @ [[Event e]\<^sub>E] @ \<sigma>)}"
-    (*add_pretocks {x. x \<noteq> Event e \<and> x \<noteq> Tock} ({[], [[Event e]\<^sub>E]} \<union> {t. \<exists> Y. Tock \<notin> Y \<and> Event e \<notin> Y \<and> t = [[Y]\<^sub>R]})*)
 
 lemma PrefixCTT_wf: "\<forall> t\<in>P. cttWF t \<Longrightarrow> \<forall> t\<in>PrefixCTT e P. cttWF t"
   unfolding PrefixCTT_def by (auto simp add: tocks_wf tocks_append_wf)
@@ -356,5 +354,321 @@ next
     using CT3_append CT3_trace.simps(2) cttWF.simps(2) apply blast
     by (metis (no_types, lifting) CT3_append CT3_trace.simps(2) CT3_trace.simps(4) CT_wf assms cttWF.elims(2) cttWF.simps(4)) 
 qed
+
+definition TockPrefixCTT :: "'e cttobs list set \<Rightarrow> 'e cttobs list set" ("tock \<rightarrow>\<^sub>C _") where
+  "TockPrefixCTT P = {t. \<exists> s\<in>tocks({x. x \<noteq> Tock \<and> x \<noteq> Tock}). t = s \<or> (\<exists> X. Tock \<notin> X \<and> Tock \<notin> X \<and> t = s @ [[X]\<^sub>R])}
+     \<union> {t. \<exists> s\<in>tocks({x. x \<noteq> Tock \<and> x \<noteq> Tock}). t = s \<or> (\<exists> \<sigma>\<in>P. \<exists> X. Tock \<notin> X \<and> t = s @ [[X]\<^sub>R, [Tock]\<^sub>E] @ \<sigma>)}"
+
+lemma TockPrefixCTT_wf: "(\<forall> t\<in>P. cttWF t) \<Longrightarrow> \<forall> t\<in>(tock \<rightarrow>\<^sub>C P). cttWF t"
+  unfolding TockPrefixCTT_def using tocks_wf apply auto
+  using cttWF.simps(2) cttWF.simps(5) tocks_append_wf by blast+
+
+lemma CT0_TockPrefixCTT: "CT0 P \<Longrightarrow> CT0 (tock \<rightarrow>\<^sub>C P)"
+  unfolding TockPrefixCTT_def CT0_def apply auto
+  using tocks.simps by blast
+
+lemma CT1_TockPrefixCTT:
+  assumes "CT1 P"
+  shows "CT1 (tock \<rightarrow>\<^sub>C P)"
+  unfolding CT1_def TockPrefixCTT_def
+proof auto
+  fix \<rho> s :: "'a cttobs list"
+  show "\<rho> \<lesssim>\<^sub>C s \<Longrightarrow> s \<in> tocks {x. x \<noteq> Tock} \<Longrightarrow>
+    \<forall>s\<in>tocks {x. x \<noteq> Tock}. \<rho> \<noteq> s \<and> (\<forall>\<sigma>\<in>P. \<forall>X. Tock \<in> X \<or> \<rho> \<noteq> s @ [X]\<^sub>R # [Tock]\<^sub>E # \<sigma>) \<Longrightarrow>
+    \<exists>s\<in>tocks {x. x \<noteq> Tock}. \<exists>X. Tock \<notin> X \<and> \<rho> = s @ [[X]\<^sub>R]"
+    using ctt_prefix_subset_tocks2[where s=s, where t=\<rho>, where X="{x. x \<noteq> Tock}"] by auto
+next
+  fix \<rho> s X
+  show "\<rho> \<lesssim>\<^sub>C s @ [[X]\<^sub>R] \<Longrightarrow>
+    \<forall>s\<in>tocks {x. x \<noteq> Tock}. \<rho> \<noteq> s \<and> (\<forall>\<sigma>\<in>P. \<forall>X. Tock \<in> X \<or> \<rho> \<noteq> s @ [X]\<^sub>R # [Tock]\<^sub>E # \<sigma>) \<Longrightarrow>
+    s \<in> tocks {x. x \<noteq> Tock} \<Longrightarrow> Tock \<notin> X \<Longrightarrow> \<exists>s\<in>tocks {x. x \<noteq> Tock}. \<exists>X. Tock \<notin> X \<and> \<rho> = s @ [[X]\<^sub>R]"
+    using ctt_prefix_subset_tocks_refusal2[where s=s, where \<rho>=\<rho>, where X="{x. x \<noteq> Tock}", where Y=X] by auto
+next
+  fix \<rho> s
+  show "\<rho> \<lesssim>\<^sub>C s \<Longrightarrow>
+    \<forall>s\<in>tocks {x. x \<noteq> Tock}. \<rho> \<noteq> s \<and> (\<forall>\<sigma>\<in>P. \<forall>X. Tock \<in> X \<or> \<rho> \<noteq> s @ [X]\<^sub>R # [Tock]\<^sub>E # \<sigma>) \<Longrightarrow>
+    s \<in> tocks {x. x \<noteq> Tock} \<Longrightarrow> \<exists>s\<in>tocks {x. x \<noteq> Tock}. \<exists>X. Tock \<notin> X \<and> \<rho> = s @ [[X]\<^sub>R]"
+    using ctt_prefix_subset_tocks2[where s=s, where t=\<rho>, where X="{x. x \<noteq> Tock}"] by auto
+next
+  fix \<rho> s \<sigma>' X
+  assume case_assms: "\<rho> \<lesssim>\<^sub>C s @ [X]\<^sub>R # [Tock]\<^sub>E # \<sigma>'" "s \<in> tocks {x. x \<noteq> Tock}" "\<sigma>' \<in> P" "Tock \<notin> X"
+  have "\<rho> \<lesssim>\<^sub>C s @ [[X]\<^sub>R, [Tock]\<^sub>E] \<or> (\<exists>t'. t' \<lesssim>\<^sub>C \<sigma>' \<and> \<rho> \<subseteq>\<^sub>C (s @ [[X]\<^sub>R, [Tock]\<^sub>E]) @ t')"
+    using case_assms ctt_prefix_subset_concat[where r="\<rho>", where s="s @ [[X]\<^sub>R, [Tock]\<^sub>E]", where t=\<sigma>'] by auto
+  then show "\<forall>s\<in>tocks {x. x \<noteq> Tock}. \<rho> \<noteq> s \<and> (\<forall>\<sigma>\<in>P. \<forall>X. Tock \<in> X \<or> \<rho> \<noteq> s @ [X]\<^sub>R # [Tock]\<^sub>E # \<sigma>) \<Longrightarrow>
+    \<exists>s\<in>tocks {x. x \<noteq> Tock}. \<exists>X. Tock \<notin> X \<and> \<rho> = s @ [[X]\<^sub>R]"
+  proof auto
+    have "s @ [[X]\<^sub>R, [Tock]\<^sub>E] \<in> tocks {x. x \<noteq> Tock}"
+      by (metis (mono_tags, lifting) case_assms(2) case_assms(4) mem_Collect_eq subsetI tocks.simps tocks_append_tocks)
+    then show "\<forall>s\<in>tocks {x. x \<noteq> Tock}. \<rho> \<noteq> s \<and> (\<forall>\<sigma>\<in>P. \<forall>X. Tock \<in> X \<or> \<rho> \<noteq> s @ [X]\<^sub>R # [Tock]\<^sub>E # \<sigma>) \<Longrightarrow>
+      \<rho> \<lesssim>\<^sub>C s @ [[X]\<^sub>R, [Tock]\<^sub>E] \<Longrightarrow> \<exists>s\<in>tocks {x. x \<noteq> Tock}. \<exists>X. Tock \<notin> X \<and> \<rho> = s @ [[X]\<^sub>R]"
+      using ctt_prefix_subset_tocks2[where s="s @ [[X]\<^sub>R, [Tock]\<^sub>E]", where t=\<rho>, where X="{x. x \<noteq> Tock}"] by auto
+  next
+    fix t'
+    assume case_assms2: "t' \<lesssim>\<^sub>C \<sigma>'" "\<rho> \<subseteq>\<^sub>C s @ [X]\<^sub>R # [Tock]\<^sub>E # t'"
+    then obtain s' t'' Y where obtain1:  "\<rho> = s' @ t'' \<and> s' \<subseteq>\<^sub>C s @ [[X]\<^sub>R, [Tock]\<^sub>E] \<and> t'' \<subseteq>\<^sub>C t'"
+      using ctt_subset_split[where r=\<rho>, where s="s @ [[X]\<^sub>R, [Tock]\<^sub>E]", where t=t'] by auto
+    then obtain s'' Y where obtain2: "s' = s'' @ [[Y]\<^sub>R, [Tock]\<^sub>E] \<and> s'' \<subseteq>\<^sub>C s \<and> Y \<subseteq> X"
+      using ctt_subset_split[where r=s', where s=s, where t="[[X]\<^sub>R, [Tock]\<^sub>E]"] apply auto
+      by (case_tac t'a rule:cttWF.cases, auto, metis ctt_subset.simps(6) neq_Nil_conv)
+    have "t'' \<in> P"
+      by (meson CT1_def assms case_assms(3) case_assms2(1) ctt_subset_imp_prefix_subset obtain1)
+    then show "\<forall>s\<in>tocks {x. x \<noteq> Tock}. \<rho> \<noteq> s \<and> (\<forall>\<sigma>\<in>P. \<forall>X. Tock \<in> X \<or> \<rho> \<noteq> s @ [X]\<^sub>R # [Tock]\<^sub>E # \<sigma>) \<Longrightarrow>
+      \<exists>s\<in>tocks {x. x \<noteq> Tock}. \<exists>X. Tock \<notin> X \<and> \<rho> = s @ [[X]\<^sub>R]"
+      by (smt obtain2 append.assoc append_Cons case_assms(2) case_assms(4) contra_subsetD ctt_subset_in_tocks obtain1 self_append_conv2)
+  qed
+qed
+
+thm TockPrefixCTT_def
+
+lemma CT2s_TockPrefix: 
+  assumes "CT2s P"
+  shows "CT2s (tock \<rightarrow>\<^sub>C P)"
+  unfolding CT2s_def
+proof auto
+  fix \<rho> \<sigma> X Y
+  assume assm1: "\<rho> @ [X]\<^sub>R # \<sigma> \<in> tock \<rightarrow>\<^sub>C P"
+  assume assm2: "Y \<inter> {e. e \<noteq> Tock \<and> \<rho> @ [[e]\<^sub>E] \<in> tock \<rightarrow>\<^sub>C P \<or> e = Tock \<and> \<rho> @ [[X]\<^sub>R, [e]\<^sub>E] \<in> tock \<rightarrow>\<^sub>C P} = {}"
+  show "\<rho> @ [X \<union> Y]\<^sub>R # \<sigma> \<in> tock \<rightarrow>\<^sub>C P"
+    using assm1 unfolding TockPrefixCTT_def
+  proof auto
+    assume case_assms: "\<rho> @ [X]\<^sub>R # \<sigma> \<in> tocks {x. x \<noteq> Tock}"
+    then have 1: "\<rho> \<in> tocks {x. x \<noteq> Tock}"
+      using tocks_mid_refusal_front_in_tocks by blast
+    then have "Tock \<in> {ea. ea \<noteq> Tock \<and> \<rho> @ [[ea]\<^sub>E] \<in> tock \<rightarrow>\<^sub>C P \<or> ea = Tock \<and> \<rho> @ [[X]\<^sub>R, [ea]\<^sub>E] \<in> tock \<rightarrow>\<^sub>C P}"
+      unfolding TockPrefixCTT_def apply auto
+      by (metis (no_types, lifting) case_assms tocks.empty_in_tocks tocks.tock_insert_in_tocks tocks_append_tocks tocks_mid_refusal)
+    then have 2: "Tock \<notin> Y"
+      using assm2 by blast
+    then have "Tock \<in> {ea. ea \<noteq> Tock \<and> \<rho> @ [[ea]\<^sub>E] \<in> tock \<rightarrow>\<^sub>C P \<or> ea = Tock \<and> \<rho> @ [[X]\<^sub>R, [ea]\<^sub>E] \<in> tock \<rightarrow>\<^sub>C P}"
+      using 1 unfolding TockPrefixCTT_def apply auto
+      by (metis case_assms tocks.empty_in_tocks tocks.tock_insert_in_tocks tocks_append_tocks tocks_mid_refusal)
+    have 3: "Tock \<notin> X"
+      using case_assms tocks_mid_refusal by fastforce
+    then have "X \<union> Y \<subseteq> {x. x \<noteq> Tock}"
+      using 1 2 3 by auto
+    then show "\<forall>s\<in>tocks {x. x \<noteq> Tock}. \<rho> @ [X \<union> Y]\<^sub>R # \<sigma> \<noteq> s \<and> (\<forall>\<sigma>'\<in>P. \<forall>Xa. Tock \<in> Xa \<or> \<rho> @ [X \<union> Y]\<^sub>R # \<sigma> \<noteq> s @ [Xa]\<^sub>R # [Tock]\<^sub>E # \<sigma>') \<Longrightarrow>
+      \<exists>s\<in>tocks {x. x \<noteq> Tock}. \<exists>Xa. Tock \<notin> Xa \<and> \<rho> @ [X \<union> Y]\<^sub>R # \<sigma> = s @ [[Xa]\<^sub>R]"
+      using case_assms apply (erule_tac x="\<rho> @ [X \<union> Y]\<^sub>R # \<sigma>" in ballE, auto)
+      using tocks_mid_refusal_change by fastforce
+  next
+    assume case_assms: "\<rho> @ [X]\<^sub>R # \<sigma> \<in> tocks {x. x \<noteq> Tock}"
+    then have 1: "\<rho> \<in> tocks {x. x \<noteq> Tock}"
+      using tocks_mid_refusal_front_in_tocks by blast
+    then have "Tock \<in> {ea. ea \<noteq> Tock \<and> \<rho> @ [[ea]\<^sub>E] \<in> tock \<rightarrow>\<^sub>C P \<or> ea = Tock \<and> \<rho> @ [[X]\<^sub>R, [ea]\<^sub>E] \<in> tock \<rightarrow>\<^sub>C P}"
+      unfolding TockPrefixCTT_def apply auto
+      by (metis (no_types, lifting) case_assms tocks.empty_in_tocks tocks.tock_insert_in_tocks tocks_append_tocks tocks_mid_refusal)
+    then have 2: "Tock \<notin> Y"
+      using assm2 by blast
+    have 3: "Tock \<notin> X"
+      using case_assms tocks_mid_refusal by fastforce
+    then have "X \<union> Y \<subseteq> {x. x \<noteq> Tock}"
+      using 1 2 3 by auto
+    then show "\<forall>s\<in>tocks {x. x \<noteq> Tock}. \<rho> @ [X \<union> Y]\<^sub>R # \<sigma> \<noteq> s \<and> (\<forall>\<sigma>'\<in>P. \<forall>Xa. Tock \<in> Xa \<or> \<rho> @ [X \<union> Y]\<^sub>R # \<sigma> \<noteq> s @ [Xa]\<^sub>R # [Tock]\<^sub>E # \<sigma>') \<Longrightarrow>
+      \<rho> @ [X]\<^sub>R # \<sigma> \<in> tocks {x. x \<noteq> Tock} \<Longrightarrow> \<exists>s\<in>tocks {x. x \<noteq> Tock}. \<exists>Xa. Tock \<notin> Xa \<and> \<rho> @ [X \<union> Y]\<^sub>R # \<sigma> = s @ [[Xa]\<^sub>R]"
+      using case_assms apply (erule_tac x="\<rho> @ [X \<union> Y]\<^sub>R # \<sigma>" in ballE, auto)
+      using tocks_mid_refusal_change by fastforce
+  next
+    fix s Xa
+    assume case_assms: "s \<in> tocks {x. x \<noteq> Tock}" "Tock \<notin> Xa" "\<rho> @ [X]\<^sub>R # \<sigma> = s @ [[Xa]\<^sub>R]"
+    then have "(\<exists> \<sigma>'. s = \<rho> @ [X]\<^sub>R # \<sigma>') \<or> (s = \<rho> \<and> X = Xa \<and> \<sigma> = [])"
+      by (metis append.right_neutral butlast.simps(2) butlast_append cttobs.inject(2) last_snoc list.distinct(1))
+    then show "\<exists>s\<in>tocks {x. x \<noteq> Tock}. \<exists>Xa. Tock \<notin> Xa \<and> \<rho> @ [X \<union> Y]\<^sub>R # \<sigma> = s @ [[Xa]\<^sub>R]"
+      using case_assms
+    proof auto
+      fix \<sigma>'
+      assume case_assms2: "s = \<rho> @ [X]\<^sub>R # \<sigma>'"
+      have 1: "\<rho> \<in> tocks {x. x \<noteq> Tock}"
+        using case_assms(1) case_assms2 tocks_mid_refusal_front_in_tocks by auto
+      have "Tock \<in> {ea. ea \<noteq> Tock \<and> \<rho> @ [[ea]\<^sub>E] \<in> tock \<rightarrow>\<^sub>C P \<or> ea = Tock \<and> \<rho> @ [[X]\<^sub>R, [ea]\<^sub>E] \<in> tock \<rightarrow>\<^sub>C P}"
+         unfolding TockPrefixCTT_def apply auto
+         using case_assms case_assms2 1 by (simp add: empty_in_tocks tock_insert_in_tocks tocks_append_tocks tocks_mid_refusal)
+       then have 2:"Tock \<notin> Y"
+         using assm2 by auto
+      have 3: "Tock \<notin> X"
+        using case_assms(1) case_assms2 tocks_mid_refusal by fastforce
+      have "X \<union> Y \<subseteq> {x. x \<noteq> Tock}"
+        using 2 3 by auto
+      then show "\<rho> @ [X \<union> Y]\<^sub>R # \<sigma>' \<in> tocks {x. x \<noteq> Tock}"
+        using case_assms case_assms2 tocks_mid_refusal_change by fastforce
+    next
+      assume "\<rho> \<in> tocks {x. x \<noteq> Tock}" "s = \<rho>" "X = Xa" "\<sigma> = []"
+      then have "Tock \<in> {ea. ea \<noteq> Tock \<and> \<rho> @ [[ea]\<^sub>E] \<in> tock \<rightarrow>\<^sub>C P \<or> ea = Tock \<and> \<rho> @ [[X]\<^sub>R, [ea]\<^sub>E] \<in> tock \<rightarrow>\<^sub>C P}"
+         unfolding TockPrefixCTT_def using case_assms apply auto
+         by (metis (mono_tags, lifting) CollectI subsetI tocks.empty_in_tocks tocks.tock_insert_in_tocks tocks_append_tocks)
+       then show "Tock \<in> Y \<Longrightarrow> False"
+         using assm2 by auto
+    qed
+  next
+    fix s \<sigma>' Xa
+    assume case_assms: "s \<in> tocks {x. x \<noteq> Tock}" "\<sigma>' \<in> P" "\<rho> @ [X]\<^sub>R # \<sigma> = s @ [Xa]\<^sub>R # [Tock]\<^sub>E # \<sigma>'" "Tock \<notin> Xa"
+    then have "(\<exists>t2'. \<rho> = (s @ [[Xa]\<^sub>R]) @ [Tock]\<^sub>E # t2' \<and> t2' \<le>\<^sub>C \<sigma>') \<or> (\<exists>s2'. s @ [[Xa]\<^sub>R] = \<rho> @ [X]\<^sub>R # s2' \<and> s2' \<le>\<^sub>C \<sigma>)"
+      using event_refusal_split[where ?s1.0=\<rho>, where ?s2.0=\<sigma>, where X=X, where ?t1.0="s @ [[Xa]\<^sub>R]", where e=Tock, where ?t2.0=\<sigma>']
+      by (simp)
+    then show "\<forall>s\<in>tocks {x. x \<noteq> Tock}.
+        \<rho> @ [X \<union> Y]\<^sub>R # \<sigma> \<noteq> s \<and> (\<forall>\<sigma>'\<in>P. \<forall>Xa. Tock \<in> Xa \<or> \<rho> @ [X \<union> Y]\<^sub>R # \<sigma> \<noteq> s @ [Xa]\<^sub>R # [Tock]\<^sub>E # \<sigma>') \<Longrightarrow>
+      \<rho> @ [X]\<^sub>R # \<sigma> = s @ [Xa]\<^sub>R # [Tock]\<^sub>E # \<sigma>' \<Longrightarrow> \<exists>s\<in>tocks {x. x \<noteq> Tock}. \<exists>Xa. Tock \<notin> Xa \<and> \<rho> @ [X \<union> Y]\<^sub>R # \<sigma> = s @ [[Xa]\<^sub>R]"
+    proof auto
+      fix t2'
+      assume case_assms2: "\<rho> = s @ [Xa]\<^sub>R # [Tock]\<^sub>E # t2'" "\<sigma>' = t2' @ [X]\<^sub>R # \<sigma>"
+      then have "{ea. ea \<noteq> Tock \<and> t2' @ [[ea]\<^sub>E] \<in> P \<or> ea = Tock \<and> t2' @ [[X]\<^sub>R, [ea]\<^sub>E] \<in> P}
+        \<subseteq> {ea. ea \<noteq> Tock \<and> \<rho> @ [[ea]\<^sub>E] \<in> tock \<rightarrow>\<^sub>C P \<or> ea = Tock \<and> \<rho> @ [[X]\<^sub>R, [ea]\<^sub>E] \<in> tock \<rightarrow>\<^sub>C P}"
+      proof auto
+        fix x :: "'a cttevent"
+        assume "\<rho> = s @ [Xa]\<^sub>R # [Tock]\<^sub>E # t2'" "\<sigma>' = t2' @ [X]\<^sub>R # \<sigma>" "t2' @ [[x]\<^sub>E] \<in> P" "x \<noteq> Tock"
+        then show "s @ [Xa]\<^sub>R # [Tock]\<^sub>E # t2' @ [[x]\<^sub>E] \<in> tock \<rightarrow>\<^sub>C P"
+          unfolding TockPrefixCTT_def using case_assms by auto
+      next
+        fix x :: "'a cttevent"
+        assume "\<rho> = s @ [Xa]\<^sub>R # [Tock]\<^sub>E # t2'" "\<sigma>' = t2' @ [X]\<^sub>R # \<sigma>" "t2' @ [[x]\<^sub>E] \<in> P" "x \<noteq> Tock"
+        then show "s @ [Xa]\<^sub>R # [Tock]\<^sub>E # t2' @ [[x]\<^sub>E] \<in> tock \<rightarrow>\<^sub>C P"
+          unfolding TockPrefixCTT_def using case_assms by auto
+      next
+        assume "\<rho> = s @ [Xa]\<^sub>R # [Tock]\<^sub>E # t2'" "t2' @ [[X]\<^sub>R, [Tock]\<^sub>E] \<in> P"
+        then show "s @ [Xa]\<^sub>R # [Tock]\<^sub>E # t2' @ [[X]\<^sub>R, [Tock]\<^sub>E] \<notin> tock \<rightarrow>\<^sub>C P \<Longrightarrow> False"
+          unfolding TockPrefixCTT_def using case_assms by auto
+      next
+        assume "\<rho> = s @ [Xa]\<^sub>R # [Tock]\<^sub>E # t2'" "t2' @ [[X]\<^sub>R, [Tock]\<^sub>E] \<in> P"
+        then show "s @ [Xa]\<^sub>R # [Tock]\<^sub>E # t2' @ [[X]\<^sub>R, [Tock]\<^sub>E] \<notin> tock \<rightarrow>\<^sub>C P \<Longrightarrow>
+          s @ [Xa]\<^sub>R # [Tock]\<^sub>E # t2' @ [[Tock]\<^sub>E] \<in> tock \<rightarrow>\<^sub>C P"
+          unfolding TockPrefixCTT_def using case_assms by auto
+      qed
+      then have 1: "Y \<inter> {ea. ea \<noteq> Tock \<and> t2' @ [[ea]\<^sub>E] \<in> P \<or> ea = Tock \<and> t2' @ [[X]\<^sub>R, [ea]\<^sub>E] \<in> P} = {}"
+        using assm2 subsetCE by auto
+      have 2: "t2' @ [X]\<^sub>R # \<sigma> \<in> P"
+        using case_assms(2) case_assms2 by auto
+      have "t2' @ [X \<union> Y]\<^sub>R # \<sigma> \<in> P"
+        using 1 2 assms unfolding CT2s_def by auto
+      then show "\<forall>sa\<in>tocks {x. x \<noteq> Tock}. s @ [Xa]\<^sub>R # [Tock]\<^sub>E # t2' @ [X \<union> Y]\<^sub>R # \<sigma> \<noteq> sa \<and>
+          (\<forall>\<sigma>'\<in>P. \<forall>Xaa. Tock \<in> Xaa \<or> s @ [Xa]\<^sub>R # [Tock]\<^sub>E # t2' @ [X \<union> Y]\<^sub>R # \<sigma> \<noteq> sa @ [Xaa]\<^sub>R # [Tock]\<^sub>E # \<sigma>') \<Longrightarrow>
+        \<exists>sa\<in>tocks {x. x \<noteq> Tock}. \<exists>Xaa. Tock \<notin> Xaa \<and> s @ [Xa]\<^sub>R # [Tock]\<^sub>E # t2' @ [X \<union> Y]\<^sub>R # \<sigma> = sa @ [[Xaa]\<^sub>R]"
+        using case_assms case_assms2 by blast
+    next
+      fix s2'
+      assume case_assms2: "\<rho> @ [X]\<^sub>R # \<sigma> = s @ [Xa]\<^sub>R # [Tock]\<^sub>E # \<sigma>'" "s @ [[Xa]\<^sub>R] = \<rho> @ [X]\<^sub>R # s2'" "s2' \<le>\<^sub>C \<sigma>"
+      obtain s2'' where s2''_cases: "s2' = s2'' @ [[Xa]\<^sub>R] \<or> (s2' = [] \<and> Xa = X)"
+        by (metis append_butlast_last_id case_assms2(2) cttobs.inject(2) last.simps last_appendR list.distinct(1))
+      then have 1: "\<rho> @ [X]\<^sub>R # s2'' \<in> tocks {x. x \<noteq> Tock} \<or> \<rho> \<in> tocks {x. x \<noteq> Tock}"
+        using case_assms case_assms2 by auto
+      then have 2: "\<rho> \<in> tocks {x. x \<noteq> Tock}"
+        using tocks_mid_refusal_front_in_tocks by auto
+      have 3: "\<rho> @ [[X]\<^sub>R, [Tock]\<^sub>E] \<in> tock \<rightarrow>\<^sub>C P"
+        unfolding TockPrefixCTT_def using s2''_cases apply auto
+        apply (metis (no_types, lifting) "2" Nil_is_append_conv butlast.simps(2) butlast_append butlast_snoc case_assms(1) case_assms2(2) tocks.empty_in_tocks tocks.tock_insert_in_tocks tocks_append_tocks tocks_mid_refusal)
+        by (metis (mono_tags, lifting) "2" CollectI case_assms(4) subsetI tocks.empty_in_tocks tocks.tock_insert_in_tocks tocks_append_tocks)
+      have 5: "Y \<subseteq> {x. x \<noteq> Tock}"
+        using assm2 3 by auto
+      then have 6: "X \<union> Y \<subseteq> {x. x \<noteq> Tock}"
+        by (smt Cons_eq_appendI append_assoc append_same_eq case_assms(1) case_assms(4) case_assms2(2) mem_Collect_eq s2''_cases subsetI sup.boundedI tocks_mid_refusal)
+      show "\<forall>s\<in>tocks {x. x \<noteq> Tock}.
+          \<rho> @ [X \<union> Y]\<^sub>R # \<sigma> \<noteq> s \<and> (\<forall>\<sigma>'\<in>P. \<forall>Xa. Tock \<in> Xa \<or> \<rho> @ [X \<union> Y]\<^sub>R # \<sigma> \<noteq> s @ [Xa]\<^sub>R # [Tock]\<^sub>E # \<sigma>') \<Longrightarrow>
+        \<exists>s\<in>tocks {x. x \<noteq> Tock}. \<exists>Xa. Tock \<notin> Xa \<and> \<rho> @ [X \<union> Y]\<^sub>R # \<sigma> = s @ [[Xa]\<^sub>R]"
+        using s2''_cases
+      proof auto
+        assume case_assms3: "s2' = s2'' @ [[Xa]\<^sub>R]"
+        obtain s2''' where s2'''_def: "s2'' = [Tock]\<^sub>E # s2'''"
+          apply (cases s2'' rule:cttWF.cases, auto)
+          using case_assms(1) case_assms2(2) case_assms3 end_refusal_notin_tocks apply force
+          using "2" case_assms(1) case_assms2(2) case_assms3 cttWF.simps(2) tocks_append_wf tocks_append_wf2 apply fastforce
+          using "2" case_assms(1) case_assms2(2) case_assms3 tocks_append_nontocks tocks_wf by fastforce+
+        then have "s2''' \<in> tocks {x. x \<noteq> Tock}"
+          by (metis (no_types, lifting) "2" Nil_is_append_conv butlast.simps(2) butlast_append butlast_snoc case_assms(1) case_assms2(2) case_assms3 list.distinct(1) list.sel(3) tocks.cases tocks_append_nontocks)
+        then show "\<forall>s\<in>tocks {x. x \<noteq> Tock}.
+            \<rho> @ [X \<union> Y]\<^sub>R # \<sigma> \<noteq> s \<and> (\<forall>\<sigma>'\<in>P. \<forall>Xa. Tock \<in> Xa \<or> \<rho> @ [X \<union> Y]\<^sub>R # \<sigma> \<noteq> s @ [Xa]\<^sub>R # [Tock]\<^sub>E # \<sigma>') \<Longrightarrow>
+          \<exists>s\<in>tocks {x. x \<noteq> Tock}. \<exists>Xa. Tock \<notin> Xa \<and> \<rho> @ [X \<union> Y]\<^sub>R # \<sigma> = s @ [[Xa]\<^sub>R]"
+          apply (erule_tac x="\<rho> @ [X \<union> Y]\<^sub>R # [Tock]\<^sub>E # s2'''" in ballE, auto)
+          apply (erule_tac x="\<sigma>'" in ballE, erule_tac x="Xa" in allE, auto simp add: case_assms)
+          using case_assms2(1) case_assms2(2) case_assms3 s2'''_def apply auto
+          using "6" case_assms(1) tocks_mid_refusal_change by fastforce
+      next
+        assume case_assms3: "s2' = []" "Xa = X"
+        then show "\<forall>s\<in>tocks {x. x \<noteq> Tock}.
+            \<rho> @ [X \<union> Y]\<^sub>R # \<sigma> \<noteq> s \<and> (\<forall>\<sigma>'\<in>P. \<forall>Xa. Tock \<in> Xa \<or> \<rho> @ [X \<union> Y]\<^sub>R # \<sigma> \<noteq> s @ [Xa]\<^sub>R # [Tock]\<^sub>E # \<sigma>') \<Longrightarrow>
+          \<exists>s\<in>tocks {x. x \<noteq> Tock}. \<exists>Xa. Tock \<notin> Xa \<and> \<rho> @ [X \<union> Y]\<^sub>R # \<sigma> = s @ [[Xa]\<^sub>R]"
+          using case_assms(4) case_assms2 2 5 apply (erule_tac x="\<rho>" in ballE, auto)
+          by (erule_tac x="\<sigma>'" in ballE, auto simp add: case_assms)
+      qed
+    qed
+  qed
+qed
+
+lemma CT3_TockPrefix: 
+  assumes "CT3 P"
+  shows "CT3 (tock \<rightarrow>\<^sub>C P)"
+  unfolding TockPrefixCTT_def CT3_def
+proof (safe, simp_all)
+  show "\<And>s. s \<in> tocks {x. x \<noteq> Tock} \<Longrightarrow> CT3_trace s"
+    by (metis (mono_tags, lifting) CT3_def CT3_tocks mem_Collect_eq)
+next
+  show "\<And>s X. s \<in> tocks {x. x \<noteq> Tock} \<Longrightarrow> Tock \<notin> X \<Longrightarrow> CT3_trace (s @ [[X]\<^sub>R])"
+    by (metis (mono_tags, lifting) CT3_append CT3_def CT3_tocks CT3_trace.simps(2) cttWF.simps(2) mem_Collect_eq)
+next
+  show "\<And>s. s \<in> tocks {x. x \<noteq> Tock} \<Longrightarrow> CT3_trace s"
+    by (metis (mono_tags, lifting) CT3_def CT3_tocks mem_Collect_eq)
+next
+  fix s \<sigma> :: "'a cttobs list"
+  fix X :: "'a cttevent set"
+  assume case_assms: "s \<in> tocks {x. x \<noteq> Tock}" "\<sigma> \<in> P" "Tock \<notin> X"  
+  have "CT3_trace \<sigma>"
+    using case_assms assms unfolding CT3_def by blast
+  then show "CT3_trace (s @ [X]\<^sub>R # [Tock]\<^sub>E # \<sigma>)"
+    using case_assms(1) case_assms(3) apply - apply (induct s rule:CT3_trace.induct, simp_all add: notin_tocks)
+    using list.distinct(1) tocks.cases apply blast
+    apply (smt CT3_trace.simps(3) append_Cons list.inject list.simps(3) mem_Collect_eq subset_eq tocks.simps)
+    apply (metis cttobs.simps(4) list.inject list.simps(3) tocks.simps)
+    done
+qed
+
+lemma CT4s_TockPrefix:
+  assumes "CT4s P"
+  shows "CT4s (tock \<rightarrow>\<^sub>C P)"
+  unfolding TockPrefixCTT_def CT4s_def
+proof auto
+  fix s :: "'a cttobs list"
+  assume "s \<in> tocks {x. x \<noteq> Tock}"   
+  then have "add_Tick_refusal_trace s \<in> tocks {x. x \<noteq> Tock}"
+    by (induct s rule:tocks.induct, auto simp add: tocks.intros)
+  then show "\<forall>sa\<in>tocks {x. x \<noteq> Tock}.
+      add_Tick_refusal_trace s \<noteq> sa \<and> (\<forall>\<sigma>\<in>P. \<forall>X. Tock \<in> X \<or> add_Tick_refusal_trace s \<noteq> sa @ [X]\<^sub>R # [Tock]\<^sub>E # \<sigma>) \<Longrightarrow>
+    \<exists>sa\<in>tocks {x. x \<noteq> Tock}. \<exists>X. Tock \<notin> X \<and> add_Tick_refusal_trace s = sa @ [[X]\<^sub>R]"
+    by (erule_tac x="add_Tick_refusal_trace s" in ballE, auto)
+next
+  fix s :: "'a cttobs list"
+  fix X :: "'a cttevent set"
+  assume case_assms: "s \<in> tocks {x. x \<noteq> Tock}" "Tock \<notin> X"
+  then have "add_Tick_refusal_trace s \<in> tocks {x. x \<noteq> Tock}"
+    by (induct s rule:tocks.induct, auto simp add: tocks.intros)
+  then show "\<exists>sa\<in>tocks {x. x \<noteq> Tock}. \<exists>Xa. Tock \<notin> Xa \<and> add_Tick_refusal_trace (s @ [[X]\<^sub>R]) = sa @ [[Xa]\<^sub>R]"
+    using case_assms apply (rule_tac x="add_Tick_refusal_trace s" in bexI, rule_tac x="X \<union> {Tick}" in exI, simp_all)
+    using add_Tick_refusal_trace_end_refusal by force
+next
+  fix s :: "'a cttobs list"
+  assume "s \<in> tocks {x. x \<noteq> Tock}"   
+  then have "add_Tick_refusal_trace s \<in> tocks {x. x \<noteq> Tock}"
+    by (induct s rule:tocks.induct, auto simp add: tocks.intros)
+  then show "\<forall>sa\<in>tocks {x. x \<noteq> Tock}.
+      add_Tick_refusal_trace s \<noteq> sa \<and> (\<forall>\<sigma>\<in>P. \<forall>X. Tock \<in> X \<or> add_Tick_refusal_trace s \<noteq> sa @ [X]\<^sub>R # [Tock]\<^sub>E # \<sigma>) \<Longrightarrow>
+    \<exists>sa\<in>tocks {x. x \<noteq> Tock}. \<exists>X. Tock \<notin> X \<and> add_Tick_refusal_trace s = sa @ [[X]\<^sub>R]"
+    by (erule_tac x="add_Tick_refusal_trace s" in ballE, auto)
+next
+  fix s \<sigma> :: "'a cttobs list"
+  fix X  :: "'a cttevent set"
+  assume case_assms: "s \<in> tocks {x. x \<noteq> Tock}" "\<sigma> \<in> P" "Tock \<notin> X"
+  then have 1: "add_Tick_refusal_trace s \<in> tocks {x. x \<noteq> Tock}"
+    by (induct s rule:tocks.induct, auto simp add: tocks.intros)
+  have 2: "add_Tick_refusal_trace \<sigma> \<in> P"
+    using assms case_assms unfolding CT4s_def by auto
+  show "\<forall>sa\<in>tocks {x. x \<noteq> Tock}. add_Tick_refusal_trace (s @ [X]\<^sub>R # [Tock]\<^sub>E # \<sigma>) \<noteq> sa \<and>
+      (\<forall>\<sigma>'\<in>P. \<forall>Xa. Tock \<in> Xa \<or> add_Tick_refusal_trace (s @ [X]\<^sub>R # [Tock]\<^sub>E # \<sigma>) \<noteq> sa @ [Xa]\<^sub>R # [Tock]\<^sub>E # \<sigma>') \<Longrightarrow>
+    \<exists>sa\<in>tocks {x. x \<noteq> Tock}. \<exists>Xa. Tock \<notin> Xa \<and> add_Tick_refusal_trace (s @ [X]\<^sub>R # [Tock]\<^sub>E # \<sigma>) = sa @ [[Xa]\<^sub>R]"
+    using 1 2 case_assms(3) apply (erule_tac x="add_Tick_refusal_trace s" in ballE, auto) 
+    apply (erule_tac x="add_Tick_refusal_trace \<sigma>" in ballE, erule_tac x="X \<union> {Tick}" in allE, auto)
+    by (metis Un_commute add_Tick_refusal_trace.simps(2) add_Tick_refusal_trace.simps(3) add_Tick_refusal_trace_concat insert_is_Un)
+qed
+
+lemma CT_TockPrefix:
+  assumes "CT P" "CT2s P" "CT4s P"
+  shows "CT (tock \<rightarrow>\<^sub>C P)"
+  using assms unfolding CT_def
+  using CT0_TockPrefixCTT CT1_TockPrefixCTT CT2s_TockPrefix CT2s_imp_CT2 CT3_TockPrefix TockPrefixCTT_wf by blast
 
 end
